SimAsm/SimAsm.thy
@@ -81,8 +81,9 @@ datatype ('v,'g,'r,'a) lang =
   | Op "('v,'g,'r,'a) pred" "('v,'g,'r) op" "('v,'g,'r,'a) auxfn"
   | Seq "('v,'g,'r,'a) lang" "('v,'g,'r,'a) lang"
   | If "('v,'g,'r) bexp" "('v,'g,'r,'a) lang" "('v,'g,'r,'a) lang" "('v,'g,'r,'a) lang"  
+  | While "('v,'g,'r) bexp" "('v,'g,'r,'a) pred" "('v,'g,'r,'a) lang" "('v,'g,'r,'a) lang" 
 (*  | If "('v,'g,'r) bexp" "('v,'g,'r,'a) lang" "('v,'g,'r,'a) lang" *)
-  | While "('v,'g,'r) bexp" "('v,'g,'r,'a) pred" "('v,'g,'r,'a) lang"
+(*  | While "('v,'g,'r) bexp" "('v,'g,'r,'a) pred" "('v,'g,'r,'a) lang" *)
   | DoWhile "('v,'g,'r,'a) pred" "('v,'g,'r,'a) lang" "('v,'g,'r) bexp"
 
 
